proved simg_exp implies simg_alt_exp

ems/SimGlobalAlts.v
@@ -47,6 +47,7 @@ Section SRCSTEPS.
 
   Variable R: Type.
   Let ITR := (itree eventE R).
+  Let ARGS := (option (string * Any.t * (Any.t -> Prop) * Any.t)).
 
   (* src tau step *)
   Variant st_step (r: ITR -> Prop): ITR -> Prop :=
@@ -72,22 +73,40 @@ Section SRCSTEPS.
   | st_star_step itr (REL: st_step (fun ktr => st_star r ktr) itr): st_star r itr
   .
 
-  Definition src_step (r: (option (string * Any.t * (Any.t -> Prop) * Any.t)) -> ITR -> Prop):
+  Definition src_step (r: ARGS -> ITR -> Prop):
     ITR -> Prop :=
     fun itr =>
       (<<TAU: st_step (r None) itr>>) \/
         (<<OBS: exists arg, forall v, obs_step (arg, v) (r (Some (arg, v))) itr>>)
   .
 
-  Definition src_plus (r: (option (string * Any.t * (Any.t -> Prop) * Any.t)) -> ITR -> Prop):
-    ITR -> Prop := (st_star (fun ktr => src_step r ktr))
+  Inductive src_star (r: ARGS -> ITR -> Prop): ARGS -> ITR -> Prop :=
+  | src_star_base
+      args itr
+      (REL: r args itr)
+    :
+    src_star r args itr
+  | src_star_step_tau
+      itr
+      (REL: src_step (fun args1 ktr => src_star r args1 ktr) itr)
+    :
+    src_star r None itr
+  | src_star_step_obs
+      args0 itr
+      (REL: st_step (fun ktr => src_star r (Some args0) ktr) itr)
+    :
+    src_star r (Some args0) itr
   .
 
-  (* Definition st_plus (r: ITR -> Prop): ITR -> Prop := src_plus (fun args ktr => (args = None) /\ (r ktr)). *)
+  Definition src_plus (r: ARGS -> ITR -> Prop): ITR -> Prop :=
+    (src_step (fun args ktr => src_star r args ktr))
+  .
 
-  Definition src_star (r: (option (string * Any.t * (Any.t -> Prop) * Any.t)) -> ITR -> Prop):
-    ITR -> Prop :=
-    (st_star (fun ktr => (r None ktr) \/ (exists arg, forall v, obs_step (arg, v) (r (Some (arg, v))) ktr))).
+  (* Definition src_plus (r: (option (string * Any.t * (Any.t -> Prop) * Any.t)) -> ITR -> Prop): *)
+  (*   ITR -> Prop := (st_star (fun ktr => src_step r ktr)) *)
+  (* . *)
+
+  (* Definition st_plus (r: ITR -> Prop): ITR -> Prop := src_plus (fun args ktr => (args = None) /\ (r ktr)). *)
 
   (* properties *)
   Lemma st_step_mon
@@ -134,23 +153,55 @@ Section SRCSTEPS.
     - des. econs 2. exists arg. i. eapply obs_step_mon. 2: eauto. eauto.
   Qed.
 
+  Lemma src_star_ind2 (r: ARGS -> ITR -> Prop) (P: ARGS -> ITR -> Prop)
+        (BASE: forall args itr (REL: r args itr), P args itr)
+        (TAU: forall itr
+                (REL: src_step (fun args1 ktr => (<<STAR: src_star r args1 ktr>>) /\
+                                                (<<IH: P args1 ktr>>)) itr),
+            P None itr)
+        (OBS: forall args0 itr
+                (REL: st_step (fun ktr => (<<STAR: src_star r (Some args0) ktr>>) /\
+                                         (<<IH: P (Some args0) ktr>>)) itr),
+            P (Some args0) itr)
+    :
+    forall args itr (STAR: src_star r args itr), P args itr.
+  Proof.
+    fix IH 3. i. inv STAR. eauto.
+    - eapply TAU. inv REL.
+      + left. inv H.
+        { econs 1. split; auto. }
+        { econs 2. des. exists x. split; auto. }
+        { econs 3. i. split; auto. }
+      + des. right. exists arg. i. specialize (H v). inv H. clarify. econs; eauto.
+    - eapply OBS. inv REL.
+      { econs 1. split; auto. }
+      { econs 2. des. exists x. split; auto. }
+      { econs 3. i. split; auto. }
+  Qed.
+
+  Lemma src_star_mon
+        (r0 r1: (option (string * Any.t * (Any.t -> Prop) * Any.t)) -> ITR -> Prop)
+        args itr
+        (MON: forall args itr, (r0 args itr) -> (r1 args itr))
+    :
+    (src_star r0 args itr) -> (src_star r1 args itr).
+  Proof.
+    i. induction H using src_star_ind2. econs 1; eauto.
+    - econs 2. eapply src_step_mon. 2: eauto. i; ss. des. auto.
+    - econs 3. eapply st_step_mon. 2: eauto. i; ss. des. auto.
+  Qed.
+
   Lemma src_plus_mon
         (r0 r1: (option (string * Any.t * (Any.t -> Prop) * Any.t)) -> ITR -> Prop) itr
         (MON: forall args itr, (r0 args itr) -> (r1 args itr))
     :
     (src_plus r0 itr) -> (src_plus r1 itr).
   Proof.
-    i. eapply st_star_mon. 2: eauto. i; ss. eapply src_step_mon. 2: eauto. eauto.
-  Qed.
-
-  Lemma src_star_mon
-        (r0 r1: (option (string * Any.t * (Any.t -> Prop) * Any.t)) -> ITR -> Prop) itr
-        (MON: forall args itr, (r0 args itr) -> (r1 args itr))
-    :
-    (src_star r0 itr) -> (src_star r1 itr).
-  Proof.
-    i. eapply st_star_mon. 2: eauto. i; ss. des; eauto. right.
-    eexists. i. eapply obs_step_mon. 2: eauto. eauto.
+    i. inv H.
+    - econs 1. eapply st_step_mon. 2: eauto. i; ss.
+      eapply src_star_mon. 2: eauto. i; ss. auto.
+    - des. econs 2. exists arg. i. eapply obs_step_mon. 2: eauto. i; ss.
+      eapply src_star_mon. 2: eauto. i; ss. auto.
   Qed.
 
 End SRCSTEPS.
@@ -159,6 +210,7 @@ Section TGTSTEPS.
 
   Variable R: Type.
   Let ITR := (itree eventE R).
+  Let ARGS := (option (string * Any.t * (Any.t -> Prop) * Any.t)).
 
   (* tgt tau step *)
   Variant tt_step (r: ITR -> Prop): ITR -> Prop :=
@@ -191,9 +243,31 @@ Section TGTSTEPS.
         (<<OBS: exists arg, forall v, obs_step (arg, v) (r (Some (arg, v))) itr>>)
   .
 
-  Definition tgt_plus (r: (option (string * Any.t * (Any.t -> Prop) * Any.t)) -> ITR -> Prop):
-    ITR -> Prop := (tt_star (fun ktr => tgt_step r ktr))
+  Inductive tgt_star (r: ARGS -> ITR -> Prop): ARGS -> ITR -> Prop :=
+  | tgt_star_base
+      args itr
+      (REL: r args itr)
+    :
+    tgt_star r args itr
+  | tgt_star_step_tau
+      itr
+      (REL: tgt_step (fun args1 ktr => tgt_star r args1 ktr) itr)
+    :
+    tgt_star r None itr
+  | tgt_star_step_obs
+      args0 itr
+      (REL: tt_step (fun ktr => tgt_star r (Some args0) ktr) itr)
+    :
+    tgt_star r (Some args0) itr
   .
+
+  Definition tgt_plus (r: ARGS -> ITR -> Prop): ITR -> Prop :=
+    (tgt_step (fun args ktr => tgt_star r args ktr))
+  .
+
+  (* Definition tgt_plus (r: (option (string * Any.t * (Any.t -> Prop) * Any.t)) -> ITR -> Prop): *)
+  (*   ITR -> Prop := (tt_star (fun ktr => tgt_step r ktr)) *)
+  (* . *)
 
   (* Definition tt_plus (r: ITR -> Prop): ITR -> Prop := tgt_plus (fun args ktr => (args = None) /\ (r ktr)). *)
 
@@ -242,18 +316,58 @@ Section TGTSTEPS.
     - des. econs 2. exists arg. i. eapply obs_step_mon. 2: eauto. eauto.
   Qed.
 
+  Lemma tgt_star_ind2 (r: ARGS -> ITR -> Prop) (P: ARGS -> ITR -> Prop)
+        (BASE: forall args itr (REL: r args itr), P args itr)
+        (TAU: forall itr
+                (REL: tgt_step (fun args1 ktr => (<<STAR: tgt_star r args1 ktr>>) /\
+                                                (<<IH: P args1 ktr>>)) itr),
+            P None itr)
+        (OBS: forall args0 itr
+                (REL: tt_step (fun ktr => (<<STAR: tgt_star r (Some args0) ktr>>) /\
+                                         (<<IH: P (Some args0) ktr>>)) itr),
+            P (Some args0) itr)
+    :
+    forall args itr (STAR: tgt_star r args itr), P args itr.
+  Proof.
+    fix IH 3. i. inv STAR. eauto.
+    - eapply TAU. inv REL.
+      + left. inv H.
+        { econs 1. split; auto. }
+        { econs 2. i. split; auto. }
+        { econs 3. des. exists x. split; auto. }
+      + des. right. exists arg. i. specialize (H v). inv H. clarify. econs; eauto.
+    - eapply OBS. inv REL.
+      { econs 1. split; auto. }
+      { econs 2. i. split; auto. }
+      { econs 3. des. exists x. split; auto. }
+  Qed.
+
+  Lemma tgt_star_mon
+        (r0 r1: (option (string * Any.t * (Any.t -> Prop) * Any.t)) -> ITR -> Prop)
+        args itr
+        (MON: forall args itr, (r0 args itr) -> (r1 args itr))
+    :
+    (tgt_star r0 args itr) -> (tgt_star r1 args itr).
+  Proof.
+    i. induction H using tgt_star_ind2. econs 1; eauto.
+    - econs 2. eapply tgt_step_mon. 2: eauto. i; ss. des. auto.
+    - econs 3. eapply tt_step_mon. 2: eauto. i; ss. des. auto.
+  Qed.
+
   Lemma tgt_plus_mon
         (r0 r1: (option (string * Any.t * (Any.t -> Prop) * Any.t)) -> ITR -> Prop) itr
         (MON: forall args itr, (r0 args itr) -> (r1 args itr))
     :
     (tgt_plus r0 itr) -> (tgt_plus r1 itr).
   Proof.
-    i. eapply tt_star_mon. 2: eauto. i; ss. eapply tgt_step_mon. 2: eauto. eauto.
+    i. inv H.
+    - econs 1. eapply tt_step_mon. 2: eauto. i; ss.
+      eapply tgt_star_mon. 2: eauto. i; ss. auto.
+    - des. econs 2. exists arg. i. eapply obs_step_mon. 2: eauto. i; ss.
+      eapply tgt_star_mon. 2: eauto. i; ss. auto.
   Qed.
 
 End TGTSTEPS.
-
-
 
 Section EXP_SIM.
 
@@ -265,13 +379,16 @@ Section EXP_SIM.
     fun itr_src itr_tgt =>
       (exists rt rs, (<<TGT: is_ret rt itr_tgt>>) /\ (<<SRC: is_ret rs itr_src>>) /\ (<<RET: RR rs rt>>))
       \/
-        ((<<TGT: (tt_step (fun ktr_tgt => (st_star (fun ktr_src => exists exp0, (simg_alt_exp _ _ RR exp0 ktr_src ktr_tgt) /\ (wfo.(lt) exp0 exp)) itr_src)) itr_tgt)>>)
-         \/
-           (<<SRC: (st_step (fun ktr_src => (tt_star (fun ktr_tgt => exists exp0, (simg_alt_exp _ _ RR exp0 ktr_src ktr_tgt) /\ (wfo.(lt) exp0 exp)) itr_tgt)) itr_src)>>)
-         \/
-           (<<TPLUS: (tgt_plus (fun targ ktr_tgt => (src_plus (fun sarg ktr_src => (<<EQ: targ = sarg>>) -> exists exp0, (simg_alt_exp _ _ RR exp0 ktr_src ktr_tgt)) itr_src)) itr_tgt)>>)
-         \/
-           (<<SPLUS: (src_plus (fun sarg ktr_src => (tgt_plus (fun targ ktr_tgt => (<<EQ: sarg = targ>>) -> exists exp0, (simg_alt_exp _ _ RR exp0 ktr_src ktr_tgt)) itr_tgt)) itr_src)>>)
+        (
+          (<<TGT: (tgt_step (fun targ ktr_tgt =>
+                               (src_step (fun sarg ktr_src => (<<EQ: targ = sarg>>) -> exists exp0, (simg_alt_exp _ _ RR exp0 ktr_src ktr_tgt)) itr_src)
+                               \/ ((targ = None) /\ exists exp0, (simg_alt_exp _ _ RR exp0 itr_src ktr_tgt) /\ (wfo.(lt) exp0 exp))
+                            ) itr_tgt)>>)
+          \/
+            (<<SRC: (src_step (fun sarg ktr_src =>
+                                 (tgt_step (fun targ ktr_tgt => (<<EQ: sarg = targ>>) -> exists exp0, (simg_alt_exp _ _ RR exp0 ktr_src ktr_tgt)) itr_tgt)
+                                 \/ ((sarg = None) /\ exists exp0, (simg_alt_exp _ _ RR exp0 ktr_src itr_tgt) /\ (wfo.(lt) exp0 exp))
+                              ) itr_src)>>)
         )
   .
 
@@ -281,13 +398,15 @@ Section EXP_SIM.
   Proof.
     ii. inv IN.
     { left. eauto. }
-    right. des; [left | right; left | do 2 right; left | do 3 right].
-    { eapply tt_step_mon. 2: eauto. i; ss. eapply st_star_mon. 2: eauto. i; ss. des; eauto. }
-    { eapply st_step_mon. 2: eauto. i; ss. eapply tt_star_mon. 2: eauto. i; ss. des; eauto. }
-    { eapply tgt_plus_mon. 2: eauto. i; ss. eapply src_plus_mon. 2: eauto. i; ss.
-      specialize (H0 H1). des; eauto. }
-    { eapply src_plus_mon. 2: eauto. i; ss. eapply tgt_plus_mon. 2: eauto. i; ss.
-      specialize (H0 H1). des; eauto. }
+    right. des; [left | right].
+    { eapply tgt_step_mon. 2: eauto. i; ss. des; [left | right].
+      - eapply src_step_mon. 2: eauto. i; ss. specialize (H0 H1). des; eauto.
+      - split; eauto.
+    }
+    { eapply src_step_mon. 2: eauto. i; ss. des; [left | right].
+      - eapply tgt_step_mon. 2: eauto. i; ss. specialize (H0 H1). des; eauto.
+      - split; eauto.
+    }
   Qed.
 
   Hint Resolve simg_alt_exp_mon: paco.
@@ -299,93 +418,151 @@ Hint Resolve simg_alt_exp_mon: paco.
 Hint Resolve cpn6_wcompat: paco.
 
 
-Section EXP_SIM_AUX.
+(** star and plus steps **)
+(* Section EXP_SIM. *)
 
-  Variable wfo: WF.
+(*   Variable wfo: WF. *)
 
-  Definition _simg_alt_exp_aux
-             (simg_alt_exp_aux: forall R0 R1 (RR: R0 -> R1 -> Prop), wfo.(T) -> (itree eventE R0) -> (itree eventE R1) -> Prop)
-             {R0 R1} (RR: R0 -> R1 -> Prop) (exp: wfo.(T)): (itree eventE R0) -> (itree eventE R1) -> Prop :=
-    fun itr_src itr_tgt =>
-      (exists rt rs, (<<TGT: is_ret rt itr_tgt>>) /\ (<<SRC: is_ret rs itr_src>>) /\ (<<RET: RR rs rt>>))
-      \/
-        ((<<TGT: (tt_step (fun ktr_tgt => (st_star (fun ktr_src => exists exp0, (simg_alt_exp_aux _ _ RR exp0 ktr_src ktr_tgt) /\ (wfo.(lt) exp0 exp)) itr_src)) itr_tgt)>>)
-         \/
-           (<<SRC: (st_step (fun ktr_src => (tt_star (fun ktr_tgt => exists exp0, (simg_alt_exp_aux _ _ RR exp0 ktr_src ktr_tgt) /\ (wfo.(lt) exp0 exp)) itr_tgt)) itr_src)>>)
-         \/
-           (<<TPLUS: (tgt_plus (fun targ ktr_tgt => (src_plus (fun sarg ktr_src => (<<EQ: targ = sarg>>) -> exists exp0, (simg_alt_exp_aux _ _ RR exp0 ktr_src ktr_tgt)) itr_src)) itr_tgt)>>)
-         \/
-           (<<SPLUS: (src_plus (fun sarg ktr_src =>
-                                  match sarg with
-                                  | Some _ => (tgt_plus (fun targ ktr_tgt => (<<EQ: sarg = targ>>) -> exists exp0, (simg_alt_exp_aux _ _ RR exp0 ktr_src ktr_tgt)) itr_tgt)
-                                  | None => (src_star (fun sarg0 ktr_src0 => (tgt_plus (fun targ ktr_tgt => (<<EQ: sarg0 = targ>>) -> exists exp0, (simg_alt_exp_aux _ _ RR exp0 ktr_src0 ktr_tgt)) itr_tgt)) ktr_src)
-                                  end
-                               ) itr_src)>>)
-        )
-  .
+(*   Definition _simg_alt_exp *)
+(*              (simg_alt_exp: forall R0 R1 (RR: R0 -> R1 -> Prop), wfo.(T) -> (itree eventE R0) -> (itree eventE R1) -> Prop) *)
+(*              {R0 R1} (RR: R0 -> R1 -> Prop) (exp: wfo.(T)): (itree eventE R0) -> (itree eventE R1) -> Prop := *)
+(*     fun itr_src itr_tgt => *)
+(*       (exists rt rs, (<<TGT: is_ret rt itr_tgt>>) /\ (<<SRC: is_ret rs itr_src>>) /\ (<<RET: RR rs rt>>)) *)
+(*       \/ *)
+(*         ((<<TGT: (tt_step (fun ktr_tgt => (st_star (fun ktr_src => exists exp0, (simg_alt_exp _ _ RR exp0 ktr_src ktr_tgt) /\ (wfo.(lt) exp0 exp)) itr_src)) itr_tgt)>>) *)
+(*          \/ *)
+(*            (<<SRC: (st_step (fun ktr_src => (tt_star (fun ktr_tgt => exists exp0, (simg_alt_exp _ _ RR exp0 ktr_src ktr_tgt) /\ (wfo.(lt) exp0 exp)) itr_tgt)) itr_src)>>) *)
+(*          \/ *)
+(*            (<<TPLUS: (tgt_plus (fun targ ktr_tgt => (src_plus (fun sarg ktr_src => (<<EQ: targ = sarg>>) -> exists exp0, (simg_alt_exp _ _ RR exp0 ktr_src ktr_tgt)) itr_src)) itr_tgt)>>) *)
+(*          \/ *)
+(*            (<<SPLUS: (src_plus (fun sarg ktr_src => (tgt_plus (fun targ ktr_tgt => (<<EQ: sarg = targ>>) -> exists exp0, (simg_alt_exp _ _ RR exp0 ktr_src ktr_tgt)) itr_tgt)) itr_src)>>) *)
+(*         ) *)
+(*   . *)
 
-  Definition simg_alt_exp_aux: forall R0 R1 (RR: R0 -> R1 -> Prop), wfo.(T) -> (itree eventE R0) -> (itree eventE R1) -> Prop := paco6 _simg_alt_exp_aux bot6.
+(*   Definition simg_alt_exp: forall R0 R1 (RR: R0 -> R1 -> Prop), wfo.(T) -> (itree eventE R0) -> (itree eventE R1) -> Prop := paco6 _simg_alt_exp bot6. *)
 
-  Lemma simg_alt_exp_aux_mon: monotone6 _simg_alt_exp_aux.
-  Proof.
-    ii. inv IN.
-    { left. eauto. }
-    right. des; [left | right; left | do 2 right; left | do 3 right].
-    { eapply tt_step_mon. 2: eauto. i; ss. eapply st_star_mon. 2: eauto. i; ss. des; eauto. }
-    { eapply st_step_mon. 2: eauto. i; ss. eapply tt_star_mon. 2: eauto. i; ss. des; eauto. }
-    { eapply tgt_plus_mon. 2: eauto. i; ss. eapply src_plus_mon. 2: eauto. i; ss.
-      specialize (H0 H1). des; eauto. }
-    { eapply src_plus_mon. 2: eauto. i; ss. des_ifs.
-      - eapply tgt_plus_mon. 2: eauto. i; ss. specialize (H0 H1). des; eauto.
-      - eapply src_star_mon. 2: eauto. i; ss.
-        eapply tgt_plus_mon. 2: eauto. i; ss. specialize (H1 H2). des; eauto.
-    }
-  Qed.
+(*   Lemma simg_alt_exp_mon: monotone6 _simg_alt_exp. *)
+(*   Proof. *)
+(*     ii. inv IN. *)
+(*     { left. eauto. } *)
+(*     right. des; [left | right; left | do 2 right; left | do 3 right]. *)
+(*     { eapply tt_step_mon. 2: eauto. i; ss. eapply st_star_mon. 2: eauto. i; ss. des; eauto. } *)
+(*     { eapply st_step_mon. 2: eauto. i; ss. eapply tt_star_mon. 2: eauto. i; ss. des; eauto. } *)
+(*     { eapply tgt_plus_mon. 2: eauto. i; ss. eapply src_plus_mon. 2: eauto. i; ss. *)
+(*       specialize (H0 H1). des; eauto. } *)
+(*     { eapply src_plus_mon. 2: eauto. i; ss. eapply tgt_plus_mon. 2: eauto. i; ss. *)
+(*       specialize (H0 H1). des; eauto. } *)
+(*   Qed. *)
 
-  Hint Resolve simg_alt_exp_aux_mon: paco.
-  Hint Resolve cpn6_wcompat: paco.
+(*   Hint Resolve simg_alt_exp_mon: paco. *)
+(*   Hint Resolve cpn6_wcompat: paco. *)
 
-End EXP_SIM_AUX.
-Hint Unfold simg_alt_exp_aux.
-Hint Resolve simg_alt_exp_aux_mon: paco.
-Hint Resolve cpn6_wcompat: paco.
+(* End EXP_SIM. *)
+(* Hint Unfold simg_alt_exp. *)
+(* Hint Resolve simg_alt_exp_mon: paco. *)
+(* Hint Resolve cpn6_wcompat: paco. *)
 
 
-Section AUX2EXP.
+(* Section EXP_SIM_AUX. *)
 
-  Lemma simg_alt_exp_aux_implies_simg_alt_exp
-        R0 R1 (RR: R0 -> R1 -> Prop)
-        (itr_src: itree eventE R0)
-        (itr_tgt: itree eventE R1)
-        (wfo: WF)
-        exp
-        (SIM: simg_alt_exp_aux wfo RR exp (itr_src) (itr_tgt))
-    :
-    simg_alt_exp wfo RR exp itr_src itr_tgt.
-  Proof.
-    ginit. revert_until RR. gcofix CIH. i.
-    (* move exp before CIH. revert_until exp. pattern exp. revert exp. *)
-    (* apply (well_founded_induction wfo.(wf)). intros exp IHe. i. *)
-    punfold SIM. inv SIM; des.
-    { gstep. left. esplits; eauto. }
-    { gstep. right; left. eapply tt_step_mon. 2: eauto. i; ss.
-      eapply st_star_mon. 2: eauto. i; ss. des. esplits; eauto.
-      pclearbot. gfinal. left; eauto.
-    }
-    { gstep. do 2 right; left. eapply st_step_mon. 2: eauto. i; ss.
-      eapply tt_star_mon. 2: eauto. i; ss. des. esplits; eauto.
-      pclearbot. gfinal. left; eauto.
-    }
-    { gstep. do 3 right; left. eapply tgt_plus_mon. 2: eauto. i; ss.
-      eapply src_plus_mon. 2: eauto. i; ss. specialize (H0 H1). des. exists exp0.
-      pclearbot. gfinal. left; eauto.
-    }
-    { gstep. do 4 right.
+(*   Variable wfo: WF. *)
+
+(*   Definition _simg_alt_exp_aux *)
+(*              (simg_alt_exp_aux: forall R0 R1 (RR: R0 -> R1 -> Prop), wfo.(T) -> (itree eventE R0) -> (itree eventE R1) -> Prop) *)
+(*              {R0 R1} (RR: R0 -> R1 -> Prop) (exp: wfo.(T)): (itree eventE R0) -> (itree eventE R1) -> Prop := *)
+(*     fun itr_src itr_tgt => *)
+(*       (exists rt rs, (<<TGT: is_ret rt itr_tgt>>) /\ (<<SRC: is_ret rs itr_src>>) /\ (<<RET: RR rs rt>>)) *)
+(*       \/ *)
+(*         ((<<TGT: (tt_step (fun ktr_tgt => (st_star (fun ktr_src => exists exp0, (simg_alt_exp_aux _ _ RR exp0 ktr_src ktr_tgt) /\ (wfo.(lt) exp0 exp)) itr_src)) itr_tgt)>>) *)
+(*          \/ *)
+(*            (<<SRC: (st_step (fun ktr_src => (tt_star (fun ktr_tgt => exists exp0, (simg_alt_exp_aux _ _ RR exp0 ktr_src ktr_tgt) /\ (wfo.(lt) exp0 exp)) itr_tgt)) itr_src)>>) *)
+(*          \/ *)
+(*            (<<TPLUS: (tgt_plus (fun targ ktr_tgt => (src_plus (fun sarg ktr_src => (<<EQ: targ = sarg>>) -> exists exp0, (simg_alt_exp_aux _ _ RR exp0 ktr_src ktr_tgt)) itr_src)) itr_tgt)>>) *)
+(*          \/ *)
+(*            (<<SPLUS: (src_plus (fun sarg ktr_src => *)
+(*                                   match sarg with *)
+(*                                   | Some _ => (tgt_plus (fun targ ktr_tgt => (<<EQ: sarg = targ>>) -> exists exp0, (simg_alt_exp_aux _ _ RR exp0 ktr_src ktr_tgt)) itr_tgt) *)
+(*                                   | None => (src_star (fun sarg0 ktr_src0 => (tgt_plus (fun targ ktr_tgt => (<<EQ: sarg0 = targ>>) -> exists exp0, (simg_alt_exp_aux _ _ RR exp0 ktr_src0 ktr_tgt)) itr_tgt)) ktr_src) *)
+(*                                   end *)
+(*                                ) itr_src)>>) *)
+(*         ) *)
+(*   . *)
+
+(*   Definition simg_alt_exp_aux: forall R0 R1 (RR: R0 -> R1 -> Prop), wfo.(T) -> (itree eventE R0) -> (itree eventE R1) -> Prop := paco6 _simg_alt_exp_aux bot6. *)
+
+(*   Lemma simg_alt_exp_aux_mon: monotone6 _simg_alt_exp_aux. *)
+(*   Proof. *)
+(*     ii. inv IN. *)
+(*     { left. eauto. } *)
+(*     right. des; [left | right; left | do 2 right; left | do 3 right]. *)
+(*     { eapply tt_step_mon. 2: eauto. i; ss. eapply st_star_mon. 2: eauto. i; ss. des; eauto. } *)
+(*     { eapply st_step_mon. 2: eauto. i; ss. eapply tt_star_mon. 2: eauto. i; ss. des; eauto. } *)
+(*     { eapply tgt_plus_mon. 2: eauto. i; ss. eapply src_plus_mon. 2: eauto. i; ss. *)
+(*       specialize (H0 H1). des; eauto. } *)
+(*     { eapply src_plus_mon. 2: eauto. i; ss. des_ifs. *)
+(*       - eapply tgt_plus_mon. 2: eauto. i; ss. specialize (H0 H1). des; eauto. *)
+(*       - eapply src_star_mon. 2: eauto. i; ss. *)
+(*         eapply tgt_plus_mon. 2: eauto. i; ss. specialize (H1 H2). des; eauto. *)
+(*     } *)
+(*   Qed. *)
+
+(*   Hint Resolve simg_alt_exp_aux_mon: paco. *)
+(*   Hint Resolve cpn6_wcompat: paco. *)
+
+(* End EXP_SIM_AUX. *)
+(* Hint Unfold simg_alt_exp_aux. *)
+(* Hint Resolve simg_alt_exp_aux_mon: paco. *)
+(* Hint Resolve cpn6_wcompat: paco. *)
 
 
+(** target step **)
+(* Section AUX2EXP. *)
 
-
-End AUX2EXP.
+(*   Lemma simg_alt_exp_aux_implies_simg_alt_exp *)
+(*         R0 R1 (RR: R0 -> R1 -> Prop) *)
+(*         (itr_src: itree eventE R0) *)
+(*         (itr_tgt: itree eventE R1) *)
+(*         (wfo: WF) *)
+(*         exp *)
+(*         (SIM: simg_alt_exp_aux wfo RR exp (itr_src) (itr_tgt)) *)
+(*     : *)
+(*     simg_alt_exp wfo RR exp itr_src itr_tgt. *)
+(*   Proof. *)
+(*     ginit. revert_until RR. gcofix CIH. i. *)
+(*     (* move exp before CIH. revert_until exp. pattern exp. revert exp. *) *)
+(*     (* apply (well_founded_induction wfo.(wf)). intros exp IHe. i. *) *)
+(*     punfold SIM. inv SIM; des. *)
+(*     { gstep. left. esplits; eauto. } *)
+(*     { gstep. right; left. eapply tt_step_mon. 2: eauto. i; ss. *)
+(*       eapply st_star_mon. 2: eauto. i; ss. des. esplits; eauto. *)
+(*       pclearbot. gfinal. left; eauto. *)
+(*     } *)
+(*     { gstep. do 2 right; left. eapply st_step_mon. 2: eauto. i; ss. *)
+(*       eapply tt_star_mon. 2: eauto. i; ss. des. esplits; eauto. *)
+(*       pclearbot. gfinal. left; eauto. *)
+(*     } *)
+(*     { gstep. do 3 right; left. eapply tgt_plus_mon. 2: eauto. i; ss. *)
+(*       eapply src_plus_mon. 2: eauto. i; ss. specialize (H0 H1). des. exists exp0. *)
+(*       pclearbot. gfinal. left; eauto. *)
+(*     } *)
+(*     { gstep. do 4 right. unfold src_plus in *. induction SPLUS using st_star_ind2. *)
+(*       { unfold src_step in REL. des. *)
+(*         { inv TAU. *)
+(*           { red. unfold src_star in REL. *)
+(*             (* inv REL. *) *)
+(*             induction REL using st_star_ind2. *)
+(*             { des. *)
+(*               - econs 1. left. econs 1. eapply tgt_plus_mon. 2: eauto. i; ss. *)
+(*                 specialize (H H0). des. exists exp0. pclearbot. gfinal. left; auto. *)
+(*               - econs 2. econs 1. econs 1. right. exists arg. i. specialize (REL v). *)
+(*                 eapply obs_step_mon. 2: eauto. i; ss. eapply tgt_plus_mon. 2: eauto. i; ss. *)
+(*                 specialize (H0 H1). des. exists exp0. pclearbot. gfinal. left; auto. *)
+(*             } *)
+(*             { inv REL; des. *)
+(*               - econs 2. econs 1. auto. *)
+(*               - econs 2. econs 2. auto. *)
+(*               -  *)
+(* End AUX2EXP. *)
 
 
 (* Section EXP_SIM. *)
