ems/SimGlobalExplicit2AltExp.v
@@ -18,32 +18,124 @@ Set Implicit Arguments.
 
 Section PROOF.
 
+  Lemma src_aux
+        R0 R1 (RR: R0 -> R1 -> Prop)
+        (wf_exp : WF)
+        (wfo := option_bot_WF (prod_WF wf_exp wf_exp) : WF)
+        (r : forall x x0 : Type, (x -> x0 -> Prop) -> T wfo -> itree eventE x -> itree eventE x0 -> Prop)
+        (CIH : forall (itr_src : itree eventE R0) (itr_tgt : itree eventE R1) (f_src f_tgt : T wf_exp),
+            simg_exp wf_exp RR f_src f_tgt itr_src itr_tgt ->
+            r R0 R1 RR (Some (f_tgt, f_src)) itr_src itr_tgt)
+        (f_src0 : T wf_exp)
+        (f_tgt : T wf_exp)
+        (itr_tgt : itree eventE R1)
+        (f_src : T wf_exp)
+        (itr_src0 : itree eventE R0)
+        (f_tgt0 : T wf_exp)
+        (LT : lt wf_exp f_src0 f_src)
+        (SIM : paco7 (_simg_exp wf_exp) bot7 R0 R1 RR f_src0 f_tgt0 itr_src0 itr_tgt)
+    :
+    (tgt_step
+       (fun (targ : option (string * Any.t * (Any.t -> Prop) * Any.t)) (ktr_tgt : itree eventE R1)
+        =>
+          (None = targ) ->
+          exists exp0 : T wfo,
+            gpaco6 (_simg_alt_exp wfo) (cpn6 (_simg_alt_exp wfo)) r r R0 R1 RR exp0 itr_src0 ktr_tgt)
+       itr_tgt) \/
+      ((@eq (option (string * Any.t * (Any.t -> Prop) * Any.t)) None None) /\
+        exists exp0 : T wfo,
+          gpaco6 (_simg_alt_exp wfo) (cpn6 (_simg_alt_exp wfo)) r r R0 R1 RR exp0 itr_src0 itr_tgt /\
+            lt wfo exp0 (Some (f_tgt, f_src))).
+  Proof.
+    move f_src0 before CIH. revert_until f_src0. pattern f_src0. revert f_src0.
+    apply (well_founded_induction wf_exp.(wf)). intros f_src0 IHs. i.
+    punfold SIM. inv SIM.
+    { right. split; auto. exists None. split. gstep. left. esplits; eauto. all: econs; eauto. }
+    { right. split; auto. exists (Some (f_tgt, f_src0)). split.
+      2:{ econs. econs 2; eauto. }
+      gstep. right. right.
+      right. exists (fn, varg, rvs). i. econs; eauto. left.
+      right. exists (fn, varg, rvs). i. econs; eauto.
+      i. inversion H. specialize (SIM0 _ _ H1). destruct SIM0; clarify.
+      exists (Some (f_tgt1, f_src1)). gfinal. left. eapply CIH; eauto.
+    }
+    { pclearbot. right. split; auto. exists (Some (f_tgt, f_src0)). split.
+      2:{ econs. econs 2; eauto. }
+      gstep. do 2 right. left. econs 1. eapply IHs. eauto. auto. eauto.
+    }
+    { pclearbot. left. left. econs 1. i. exists (Some (f_tgt1, f_src1)). gfinal. left. auto. }
+    { des. pclearbot. right. split; auto. exists (Some (f_tgt, f_src0)). split.
+      2:{ econs. econs 2; eauto. }
+      gstep. do 2 right. left. econs 2. exists x. eapply IHs. eauto. auto. eauto.
+    }
+    { pclearbot. left. left. econs 2. i. specialize (SIM0 x).
+      exists (Some (f_tgt1, f_src1)). gfinal. left. auto.
+    }
+    { pclearbot. right. split; auto. exists (Some (f_tgt, f_src0)). split.
+      2:{ econs. econs 2; eauto. }
+      gstep. do 2 right. left. econs 3. i. specialize (SIM0 x). eapply IHs. eauto. auto. eauto.
+    }
+    { des. pclearbot. left. left. econs 3. exists x. i. exists (Some (f_tgt1, f_src1)). gfinal. left. auto. }
+  Qed.
+
   Theorem simg_exp_implies_simg_alt_exp
           R0 R1 (RR: R0 -> R1 -> Prop)
           (itr_src: itree eventE R0)
           (itr_tgt: itree eventE R1)
           (wf_exp: WF)
-          (e_src e_tgt: wf_exp.(T))
-          (SIM: simg_exp wf_exp RR e_src e_tgt (itr_src) (itr_tgt))
+          (f_src f_tgt: wf_exp.(T))
+          (SIM: simg_exp wf_exp RR f_src f_tgt (itr_src) (itr_tgt))
     :
     exists wfo exp,
       simg_alt_exp wfo RR exp itr_src itr_tgt.
   Proof.
-    set (wfo := prod_WF wf_exp wf_exp). Local Opaque prod_WF.
-    move wfo before RR. exists wfo. exists (e_tgt, e_src).
+    set (wfo := option_bot_WF (prod_WF wf_exp wf_exp)).
+    Local Opaque option_bot_WF prod_WF. move wfo before RR.
+    exists wfo. exists (Some (f_tgt, f_src)).
     ginit. revert_until wfo. gcofix CIH. i.
-    move e_tgt before CIH. revert_until e_tgt. pattern e_tgt. revert e_tgt.
-    apply (well_founded_induction wf_exp.(wf)). intros e_tgt IHt. i.
+    (* move f_tgt before CIH. revert_until f_tgt. pattern f_tgt. revert f_tgt. *)
+    (* apply (well_founded_induction wf_exp.(wf)). intros f_tgt IHt. i. *)
     punfold SIM. inv SIM.
     { gstep. left. esplits; eauto. all: econs; eauto. }
-    { gstep. right. do 3 right. econs 1. right. exists (fn, varg, rvs). i. econs; eauto.
-      econs 1. right. exists (fn, varg, rvs). i. econs; eauto.
-      i. inversion H. specialize (SIM0 v v0 H1). destruct SIM0; clarify.
-      exists (f_tgt0, f_src0). gfinal. left. eapply CIH; eauto.
+    { gstep. right. right.
+      right. exists (fn, varg, rvs). i. econs; eauto. left.
+      right. exists (fn, varg, rvs). i. econs; eauto.
+      i. inversion H. specialize (SIM0 _ _ H1). destruct SIM0; clarify.
+      exists (Some (f_tgt0, f_src0)). gfinal. left. eapply CIH; eauto.
     }
-    { destruct SIM0 as [SIM | SIM]; clarify. 
-
-    
-
+    { destruct SIM0 as [SIM | SIM]; clarify.
+      (* clear IHt. *)
+      gstep. do 2 right. econs 1. econs 1.
+      eapply src_aux; eauto.
+    }
+    { destruct SIM0 as [SIM | SIM]; clarify.
+      gstep. right; left. econs 1. econs 1.
+      right. split; auto. exists (Some (f_tgt0, f_src0)). split.
+      2:{ econs. econs 1; auto. }
+      gfinal. left; eauto.
+    }
+    { des. destruct SIM0 as [SIM | SIM]; clarify.
+      (* clear IHt. *)
+      gstep. do 2 right. econs 1. econs 2. exists x.
+      eapply src_aux; eauto.
+    }
+    { gstep. right; left. econs 1. econs 2. i.
+      right. split; auto. exists (Some (f_tgt0, f_src0)). split.
+      2:{ econs. econs 1; auto. }
+      destruct (SIM0 x) as [SIM | SIM]; clarify.
+      gfinal. left; eauto.
+    }
+    { gstep. do 2 right. econs 1. econs 3. i.
+      destruct (SIM0 x) as [SIM | SIM]; clarify.
+      (* clear IHt. *)
+      eapply src_aux; eauto.
+    }
+    { des. destruct SIM0 as [SIM | SIM]; clarify.
+      gstep. right; left. econs 1. econs 3. exists x.
+      right. split; auto. exists (Some (f_tgt0, f_src0)). split.
+      2:{ econs. econs 1; auto. }
+      gfinal. left; eauto.
+    }
+  Qed.
 
 End PROOF.
